src/Transforms/die.v
@@ -15,6 +15,7 @@ Require Import Maps.
 Require Import opsem_props.
 Require Import primitives.
 Require Import program_sim.
+Require Import palloca_props.
 
 Definition pure_cmd (c:cmd) : Prop :=
 match c with
@@ -190,7 +191,7 @@ Proof.
       contradict H; eauto using s_isFinialState__stuck.
 
       assert (OpsemPP.wf_State cfg1 IS1') as Hwfpp'.
-        admit. (* wf pp *)
+        apply OpsemPP.preservation in Hop1; auto.
       eapply die_is_sim in Hstsim; eauto.
       destruct Hstsim as [Hstsim1 Hstsim2].
       destruct (@die.removable_State_dec diinfo IS1) as [Hrm | Hnrm].
@@ -264,6 +265,28 @@ Qed.
 
 Lemma subst_fdef__diinfo: forall f id0 v0,
   exists diinfo:DIInfo, DI_f diinfo = subst_fdef id0 v0 f /\ DI_id diinfo = id0.
+Admitted.
+
+Lemma die_wfS: forall id0 f diinfo los nts Ps1 Ps2
+  (HwfS: wf_system nil [module_intro los nts (Ps1 ++ product_fdef f :: Ps2)])
+  (Heq1: f = DI_f diinfo) (Heq2: id0 = DI_id diinfo),
+  wf_system nil
+    [module_intro los nts (Ps1 ++  product_fdef (remove_fdef id0 f) :: Ps2)].
+Admitted.
+
+Lemma die_wfPI: forall id0 f diinfo los nts Ps1 Ps2 pinfo
+  (Hwfpi: WF_PhiInfo pinfo)
+  (HwfS: wf_system nil [module_intro los nts (Ps1 ++ product_fdef f :: Ps2)])
+  (Heq1: f = DI_f diinfo) (Heq2: id0 = DI_id diinfo) (Heq3: f = PI_f pinfo),
+  WF_PhiInfo (update_pinfo pinfo (remove_fdef id0 f)).
+Admitted.
+
+Lemma remove_successors : forall f id',
+  successors f = successors (remove_fdef id' f).
+Admitted.
+
+Lemma remove_reachablity_analysis : forall f id',
+  dtree.reachablity_analysis f = dtree.reachablity_analysis (remove_fdef id' f).
 Admitted.
 
 (*****************************)
