src/Transforms/laa.v
@@ -579,10 +579,17 @@ Lemma undefined_state__laa_State_simulation: forall pinfo laainfo cfg1 St1 cfg2
   OpsemPP.undefined_state cfg1 St1 -> OpsemPP.undefined_state cfg2 St2.
 Admitted.
 
+Lemma laainfo__substable_values: forall td gl pinfo laainfo, 
+  substable_values td gl (PI_f pinfo) (value_id (LAA_lid pinfo laainfo))
+    [!pinfo!].
+Admitted.
+
 Lemma sop_star__laa_State_simulation: forall pinfo laainfo cfg1 IS1 cfg2 IS2 tr
   FS2 (Hwfpi: WF_PhiInfo pinfo) (Hwfpp: OpsemPP.wf_State cfg1 IS1) 
   (HwfS1: id_rhs_val.wf_State (value_id (LAA_lid pinfo laainfo)) 
            [! pinfo !] (PI_f pinfo) cfg1 IS1)
+  (Hvev: vev_State (value_id (LAA_lid pinfo laainfo)) [!pinfo!] (PI_f pinfo) 
+           cfg1 IS1)
   (Hstsim : State_simulation pinfo laainfo cfg1 IS1 cfg2 IS2)
   (Hopstar : Opsem.sop_star cfg2 IS2 FS2 tr),
   exists FS1, Opsem.sop_star cfg1 IS1 FS1 tr /\ 
@@ -604,10 +611,15 @@ Proof.
       eapply laa_is_sim in Hstsim; eauto.
       destruct Hstsim as [Hstsim EQ]; subst.
       assert (OpsemPP.wf_State cfg1 IS1') as Hwfpp'.
-        admit. (* wf pp *)
+        apply OpsemPP.preservation in Hop1; auto.
       assert (id_rhs_val.wf_State (value_id (LAA_lid pinfo laainfo))
                [! pinfo !] (PI_f pinfo) cfg1 IS1') as HwfS1'.
-        admit. (* wf pp *)
+        eapply id_rhs_val.preservation in Hop1; eauto.
+          apply laainfo__substable_values.
+      assert (vev_State (value_id (LAA_lid pinfo laainfo)) [!pinfo!] 
+        (PI_f pinfo) cfg1 IS1') as Hvev'.
+        eapply vev_State__preservation in Hop1; 
+          eauto using laainfo__substable_values.
       eapply IHHopstar in Hstsim; eauto.
       destruct Hstsim as [FS1 [Hopstar1 Hstsim]].
       exists FS1.
@@ -621,6 +633,8 @@ Lemma sop_div__laa_State_simulation: forall pinfo laainfo cfg1 IS1 cfg2 IS2 tr
   (Hwfpi: WF_PhiInfo pinfo) (Hwfpp: OpsemPP.wf_State cfg1 IS1) 
   (HwfS1: id_rhs_val.wf_State (value_id (LAA_lid pinfo laainfo)) 
             [! pinfo !] (PI_f pinfo) cfg1 IS1)
+  (Hvev: vev_State (value_id (LAA_lid pinfo laainfo)) [!pinfo!] (PI_f pinfo) 
+           cfg1 IS1)
   (Hstsim : State_simulation pinfo laainfo cfg1 IS1 cfg2 IS2)
   (Hopstar : Opsem.sop_diverges cfg2 IS2 tr),
   Opsem.sop_diverges cfg1 IS1 tr.
@@ -689,6 +703,9 @@ Proof.
     assert (id_rhs_val.wf_State (value_id (LAA_lid pinfo laainfo))
               [! pinfo !] (PI_f pinfo) cfg1 IS1) as Hisrhsval.
       eapply s_genInitState__id_rhs_val; eauto.
+    assert (vev_State (value_id (LAA_lid pinfo laainfo)) [!pinfo!] 
+      (PI_f pinfo) cfg1 IS1) as Hvev.
+      eapply s_genInitState__vev_State; eauto.
     eapply sop_star__laa_State_simulation in Hstsim; eauto.
     destruct Hstsim as [FS1 [Hopstar1 Hstsim']].
     eapply s_isFinialState__laa_State_simulation in Hstsim'; eauto.
@@ -703,10 +720,59 @@ Proof.
     assert (id_rhs_val.wf_State (value_id (LAA_lid pinfo laainfo))
               [! pinfo !] (PI_f pinfo) cfg1 IS1) as Hisrhsval.
       eapply s_genInitState__id_rhs_val; eauto.
+    assert (vev_State (value_id (LAA_lid pinfo laainfo)) [!pinfo!] 
+      (PI_f pinfo) cfg1 IS1) as Hvev.
+      eapply s_genInitState__vev_State; eauto.
     eapply sop_div__laa_State_simulation in Hstsim; eauto.
     destruct Hstsim as [FS1 Hopdiv1].
     econstructor; eauto.
 Qed.
+
+Lemma laa_wfS: forall (los : layouts) (nts : namedts) (fh : fheader) 
+  (dones : list id) (pinfo: PhiInfo)
+  (bs1 : list block) (l0 : l) (ps0 : phinodes) (cs0 : cmds) (tmn0 : terminator)
+  (bs2 : list block) (Ps1 : list product) (Ps2 : list product)
+  (v : value) (cs : cmds) (Hwfpi: WF_PhiInfo pinfo) 
+  (Hst : ret inr (v, cs) = find_init_stld cs0 (PI_id pinfo) dones)
+  (i1 : id) (Hld : ret inl i1 = find_next_stld cs (PI_id pinfo))
+  (HwfS : 
+     wf_system nil
+       [module_intro los nts 
+         (Ps1 ++ 
+          product_fdef 
+            (fdef_intro fh (bs1 ++ block_intro l0 ps0 cs0 tmn0 :: bs2))
+          :: Ps2)])
+  (Heq: PI_f pinfo = fdef_intro fh (bs1 ++ block_intro l0 ps0 cs0 tmn0 :: bs2)),
+  wf_system nil
+    [module_intro los nts 
+      (Ps1 ++ 
+       product_fdef 
+         (subst_fdef i1 v 
+           (fdef_intro fh (bs1 ++ block_intro l0 ps0 cs0 tmn0 :: bs2))) :: Ps2)].
+Proof.
+Admitted.
+
+Lemma laa_wfPI: forall (los : layouts) (nts : namedts) (fh : fheader) 
+  (dones : list id) (pinfo: PhiInfo)
+  (bs1 : list block) (l0 : l) (ps0 : phinodes) (cs0 : cmds) (tmn0 : terminator)
+  (bs2 : list block) (Ps1 : list product) (Ps2 : list product)
+  (v : value) (cs : cmds) (Hwfpi: WF_PhiInfo pinfo) 
+  (Hst : ret inr (v, cs) = find_init_stld cs0 (PI_id pinfo) dones)
+  (i1 : id) (Hld : ret inl i1 = find_next_stld cs (PI_id pinfo))
+  (HwfS : 
+     wf_system nil
+       [module_intro los nts 
+         (Ps1 ++ 
+          product_fdef 
+            (fdef_intro fh (bs1 ++ block_intro l0 ps0 cs0 tmn0 :: bs2))
+          :: Ps2)])
+  (Heq: PI_f pinfo = fdef_intro fh (bs1 ++ block_intro l0 ps0 cs0 tmn0 :: bs2)),
+  WF_PhiInfo 
+    (update_pinfo pinfo 
+      (subst_fdef i1 v 
+        (fdef_intro fh (bs1 ++ block_intro l0 ps0 cs0 tmn0 :: bs2)))).
+Proof.
+Admitted.
 
 (*****************************)
 (*
