src/Transforms/mem2reg_correct.v
@@ -19,6 +19,7 @@ Require Import palloca_props.
 Require Import mem2reg.
 Require Import memory_props.
 Require Import program_sim.
+Require Import subst.
 Require Import las.
 Require Import laa.
 Require Import dae.
@@ -36,7 +37,73 @@ Parameter does_phi_elim_is_true: does_phi_elim tt = true.
 
 Parameter does_stld_elim_is_true: does_stld_elim tt = true.
 
-Lemma las_die_sim: forall (los : layouts) (nts : namedts) (fh : fheader) 
+Lemma program_sim_wfS_trans: forall (P1 P2 P3 : system) (main : id) 
+  (VarArgs : list (GVsT DGVs)) (HwfS: wf_system nil P3),
+  (wf_system nil P2 -> program_sim P1 P2 main VarArgs /\ wf_system nil P1) ->
+  (wf_system nil P3 -> program_sim P2 P3 main VarArgs /\ wf_system nil P2) ->
+  program_sim P1 P3 main VarArgs /\ wf_system nil P1.
+Proof.
+  intros.
+  apply H0 in HwfS. destruct HwfS.
+  apply H in H2. destruct H2.
+  split; auto.
+  eapply program_sim_trans; eauto.
+Qed.
+
+Lemma las_die_wfPI: forall (los : layouts) (nts : namedts) (fh : fheader) 
+  (dones : list id) (pinfo: PhiInfo)
+  (bs1 : list block) (l0 : l) (ps0 : phinodes) (cs0 : cmds) (tmn0 : terminator)
+  (bs2 : list block) (Ps1 : list product) (Ps2 : list product) (i0 : id)
+  (v : value) (cs : cmds) 
+  (Hst : ret inl (i0, v, cs) = find_init_stld cs0 (PI_id pinfo) dones)
+  (i1 : id) (Hld : ret inl i1 = find_next_stld cs (PI_id pinfo))
+  (Heq: PI_f pinfo = fdef_intro fh (bs1 ++ block_intro l0 ps0 cs0 tmn0 :: bs2))
+  (Hwfpi: WF_PhiInfo pinfo) 
+  (HwfS : 
+     wf_system nil
+       [module_intro los nts 
+         (Ps1 ++ 
+          product_fdef 
+            (fdef_intro fh (bs1 ++ block_intro l0 ps0 cs0 tmn0 :: bs2))
+          :: Ps2)]),
+  WF_PhiInfo (update_pinfo pinfo 
+         (fdef_intro fh
+           (List.map (remove_block i1)
+             (List.map (subst_block i1 v) 
+               (bs1 ++ block_intro l0 ps0 cs0 tmn0 :: bs2))))).
+Proof.
+  intros.
+  assert ((fdef_intro fh
+           (List.map (remove_block i1)
+             (List.map (subst_block i1 v)
+               (bs1 ++ block_intro l0 ps0 cs0 tmn0 :: bs2)))) =
+          remove_fdef i1 
+            (subst_fdef i1 v
+              (fdef_intro fh (bs1 ++ block_intro l0 ps0 cs0 tmn0 :: bs2)))) 
+    as J.
+    simpl. auto.
+  rewrite J.
+  destruct (@subst_fdef__diinfo 
+    (fdef_intro fh (bs1 ++ block_intro l0 ps0 cs0 tmn0 :: bs2)) i1 v) as 
+    [diinfo [J1 J2]].
+  change
+    (update_pinfo pinfo
+      (remove_fdef i1
+        (subst_fdef i1 v
+          (fdef_intro fh (bs1 ++ block_intro l0 ps0 cs0 tmn0 :: bs2))))) with
+    (update_pinfo
+      (update_pinfo pinfo
+        (subst_fdef i1 v
+          (fdef_intro fh (bs1 ++ block_intro l0 ps0 cs0 tmn0 :: bs2))))
+      (remove_fdef i1
+        (subst_fdef i1 v
+          (fdef_intro fh (bs1 ++ block_intro l0 ps0 cs0 tmn0 :: bs2))))).
+  eapply die_wfPI; eauto.
+    eapply las_wfPI; eauto.
+    eapply las_wfS; eauto.
+Qed.
+
+Lemma las_die_sim_wfS: forall (los : layouts) (nts : namedts) (fh : fheader) 
   (dones : list id) (pinfo: PhiInfo) (main : id) (VarArgs : list (GVsT DGVs))
   (bs1 : list block) (l0 : l) (ps0 : phinodes) (cs0 : cmds) (tmn0 : terminator)
   (bs2 : list block) (Ps1 : list product) (Ps2 : list product) (i0 : id)
@@ -64,7 +131,15 @@ Lemma las_die_sim: forall (los : layouts) (nts : namedts) (fh : fheader)
       (Ps1 ++ 
        product_fdef (fdef_intro fh (bs1 ++ block_intro l0 ps0 cs0 tmn0 :: bs2))::
        Ps2)]
-    main VarArgs.
+    main VarArgs /\
+  wf_system nil
+    [module_intro los nts
+      (Ps1 ++
+       product_fdef
+         (fdef_intro fh
+           (List.map (remove_block i1)
+             (List.map (subst_block i1 v) 
+               (bs1 ++ block_intro l0 ps0 cs0 tmn0 :: bs2)))) :: Ps2)].
 Proof.
   intros.
   assert ((fdef_intro fh
@@ -77,22 +152,78 @@ Proof.
     as J.
     simpl. auto.
   rewrite J.
-  apply program_sim_trans with (P2:=
-    [module_intro los nts
-        (Ps1 ++
-         product_fdef
-           (subst_fdef i1 v
-              (fdef_intro fh (bs1 ++ block_intro l0 ps0 cs0 tmn0 :: bs2))) :: 
-         Ps2)]).
-    destruct (@subst_fdef__diinfo 
-      (fdef_intro fh (bs1 ++ block_intro l0 ps0 cs0 tmn0 :: bs2)) i1 v) as 
-      [diinfo [J1 J2]].
-    eapply die_sim; eauto.
-      admit. (* subst pres wfs *)  
-    eapply las_sim; eauto.
+  destruct (@subst_fdef__diinfo 
+    (fdef_intro fh (bs1 ++ block_intro l0 ps0 cs0 tmn0 :: bs2)) i1 v) as 
+    [diinfo [J1 J2]].
+  apply program_sim_wfS_trans with (P2:=
+      [module_intro los nts
+          (Ps1 ++
+           product_fdef
+             (subst_fdef i1 v
+                (fdef_intro fh (bs1 ++ block_intro l0 ps0 cs0 tmn0 :: bs2))) :: 
+           Ps2)]); auto; intros.
+    split.
+      eapply die_sim; eauto.
+      eapply die_wfS; eauto.
+    split.
+      eapply las_sim; eauto.
+      eapply las_wfS; eauto.
 Qed.
 
-Lemma laa_die_sim: forall (los : layouts) (nts : namedts) (fh : fheader) 
+Lemma laa_die_wfPI: forall (los : layouts) (nts : namedts) (fh : fheader) 
+  (dones : list id) (pinfo : PhiInfo)
+  (bs1 : list block) (l0 : l) (ps0 : phinodes) (cs0 : cmds) (tmn0 : terminator)
+  (bs2 : list block) (Ps1 : list product) (Ps2 : list product) (v : value)
+  (cs : cmds) 
+  (Hst : ret inr (v, cs) = find_init_stld cs0 (PI_id pinfo) dones)
+  (i1 : id) (Hld : ret inl i1 = find_next_stld cs (PI_id pinfo))
+  (Heq: PI_f pinfo = fdef_intro fh (bs1 ++ block_intro l0 ps0 cs0 tmn0 :: bs2))
+  (Hwfpi: WF_PhiInfo pinfo) 
+  (HwfS : 
+     wf_system nil
+       [module_intro los nts 
+         (Ps1 ++ 
+          product_fdef 
+            (fdef_intro fh (bs1 ++ block_intro l0 ps0 cs0 tmn0 :: bs2))
+          :: Ps2)]),
+  WF_PhiInfo (update_pinfo pinfo
+    (fdef_intro fh
+      (List.map (remove_block i1)
+        (List.map (subst_block i1 v)
+          (bs1 ++ block_intro l0 ps0 cs0 tmn0 :: bs2))))).
+Proof.
+  intros.
+  assert ((fdef_intro fh
+           (List.map (remove_block i1)
+             (List.map (subst_block i1 v)
+               (bs1 ++ block_intro l0 ps0 cs0 tmn0 :: bs2)))) =
+          remove_fdef i1 
+            (subst_fdef i1 v
+              (fdef_intro fh (bs1 ++ block_intro l0 ps0 cs0 tmn0 :: bs2)))) 
+    as J.
+    simpl. auto.
+  rewrite J.
+  destruct (@subst_fdef__diinfo 
+    (fdef_intro fh (bs1 ++ block_intro l0 ps0 cs0 tmn0 :: bs2)) i1 v) as 
+    [diinfo [J1 J2]].
+  change
+    (update_pinfo pinfo
+      (remove_fdef i1
+        (subst_fdef i1 v
+          (fdef_intro fh (bs1 ++ block_intro l0 ps0 cs0 tmn0 :: bs2))))) with
+    (update_pinfo
+      (update_pinfo pinfo
+        (subst_fdef i1 v
+          (fdef_intro fh (bs1 ++ block_intro l0 ps0 cs0 tmn0 :: bs2))))
+      (remove_fdef i1
+        (subst_fdef i1 v
+          (fdef_intro fh (bs1 ++ block_intro l0 ps0 cs0 tmn0 :: bs2))))).
+  eapply die_wfPI; eauto.
+    eapply laa_wfPI; eauto.
+    eapply laa_wfS; eauto.
+Qed.
+
+Lemma laa_die_sim_wfS: forall (los : layouts) (nts : namedts) (fh : fheader) 
   (dones : list id) (pinfo : PhiInfo) (main : id) (VarArgs : list (GVsT DGVs))
   (bs1 : list block) (l0 : l) (ps0 : phinodes) (cs0 : cmds) (tmn0 : terminator)
   (bs2 : list block) (Ps1 : list product) (Ps2 : list product) (v : value)
@@ -120,7 +251,15 @@ Lemma laa_die_sim: forall (los : layouts) (nts : namedts) (fh : fheader)
       (Ps1 ++
        product_fdef
          (fdef_intro fh (bs1 ++ block_intro l0 ps0 cs0 tmn0 :: bs2)) :: Ps2)]
-    main VarArgs.
+    main VarArgs /\
+  wf_system nil
+    [module_intro los nts
+      (Ps1 ++
+       product_fdef
+         (fdef_intro fh
+            (List.map (remove_block i1)
+               (List.map (subst_block i1 v)
+                  (bs1 ++ block_intro l0 ps0 cs0 tmn0 :: bs2)))) :: Ps2)].
 Proof.
   intros.
   assert ((fdef_intro fh
@@ -133,24 +272,99 @@ Proof.
     as J.
     simpl. auto.
   rewrite J.
-  apply program_sim_trans with (P2:=
-    [module_intro los nts
-        (Ps1 ++
-         product_fdef
-           (subst_fdef i1 v
-              (fdef_intro fh (bs1 ++ block_intro l0 ps0 cs0 tmn0 :: bs2))) :: 
-         Ps2)]).
-    destruct (@subst_fdef__diinfo 
-      (fdef_intro fh (bs1 ++ block_intro l0 ps0 cs0 tmn0 :: bs2)) i1 v) as 
-      [diinfo [J1 J2]].
-    eapply die_sim; eauto.
-      admit. (* subst pres wfS *)  
-
-    eapply laa_sim; eauto.
+  destruct (@subst_fdef__diinfo 
+    (fdef_intro fh (bs1 ++ block_intro l0 ps0 cs0 tmn0 :: bs2)) i1 v) as 
+    [diinfo [J1 J2]].
+  apply program_sim_wfS_trans with (P2:=
+      [module_intro los nts
+          (Ps1 ++
+           product_fdef
+             (subst_fdef i1 v
+                (fdef_intro fh (bs1 ++ block_intro l0 ps0 cs0 tmn0 :: bs2))) :: 
+           Ps2)]); auto; intros.
+    split.
+      eapply die_sim; eauto.
+      eapply die_wfS; eauto.
+    split.
+      eapply laa_sim; eauto.
+      eapply laa_wfS; eauto.
 Qed.
 
-Lemma elim_stld_cmds_sim: forall los nts fh dones (pinfo:PhiInfo) f0 dones0 main 
-  VarArgs bs1 l0 ps0 cs0 tmn0 bs2 Ps1 Ps2
+Lemma remove_subst_reachablity_successors : forall i2 i1 v1 f,
+  dtree.reachablity_analysis f = 
+    dtree.reachablity_analysis (remove_fdef i2 (subst_fdef i1 v1 f)) /\
+  successors f = successors (remove_fdef i2 (subst_fdef i1 v1 f)).
+Proof.
+  split.
+    transitivity (dtree.reachablity_analysis (subst_fdef i1 v1 f)).
+      apply subst_reachablity_analysis.
+      apply remove_reachablity_analysis.
+
+    transitivity (successors (subst_fdef i1 v1 f)).
+      apply subst_successors.
+      apply remove_successors.
+Qed.
+
+Lemma elim_stld_cmds_reachablity_successors: forall f cs0 f0 
+  dones0 dones id0 (Hpass : (f0, true, dones0) = elim_stld_cmds f cs0 id0 dones),
+  dtree.reachablity_analysis f = dtree.reachablity_analysis f0 /\
+  successors f = successors f0.
+Proof.
+  intros.
+  unfold elim_stld_cmds in Hpass.
+  remember (find_init_stld cs0 id0 dones) as R1.
+  destruct R1 as [[[[]]|[]]|]; tinv Hpass.
+    remember (find_next_stld c id0) as R2.
+    destruct R2 as [[|[]]|]; inv Hpass.
+      apply remove_subst_reachablity_successors.
+      split.
+        apply remove_reachablity_analysis.
+        apply remove_successors.
+      split; auto.
+
+    remember (find_next_stld c id0) as R2.
+    destruct R2 as [[|[]]|]; inv Hpass.
+      apply remove_subst_reachablity_successors.
+      split; auto.
+      split; auto.
+Qed.
+
+Lemma elim_stld_cmds_wfPI: forall los nts fh dones (pinfo:PhiInfo) f0 dones0 
+  bs1 l0 ps0 cs0 tmn0 bs2 Ps1 Ps2
+  (Hpass : (f0, true, dones0) =
+           elim_stld_cmds
+             (fdef_intro fh (bs1 ++ block_intro l0 ps0 cs0 tmn0 :: bs2)) cs0
+             (PI_id pinfo) dones)
+  (Heq: PI_f pinfo = fdef_intro fh (bs1 ++ block_intro l0 ps0 cs0 tmn0 :: bs2))
+  (Hwfpi: WF_PhiInfo pinfo) 
+  (HwfS : 
+     wf_system nil
+       [module_intro los nts 
+         (Ps1 ++ 
+          product_fdef 
+            (fdef_intro fh (bs1 ++ block_intro l0 ps0 cs0 tmn0 :: bs2))
+          :: Ps2)]),
+  WF_PhiInfo (update_pinfo pinfo f0).
+Proof.
+  intros.
+  unfold elim_stld_cmds in Hpass.
+  remember (find_init_stld cs0 (PI_id pinfo) dones) as R1.
+  destruct R1 as [[[[]]|[]]|]; tinv Hpass.
+    remember (find_next_stld c (PI_id pinfo)) as R2.
+    destruct R2 as [[|[]]|]; inv Hpass.
+      eapply las_die_wfPI; eauto.
+      eapply sas_wfPI; eauto.
+      rewrite <- Heq. rewrite update_pinfo_eq; auto.
+
+    remember (find_next_stld c (PI_id pinfo)) as R2.
+    destruct R2 as [[|[]]|]; inv Hpass.
+      eapply laa_die_wfPI; eauto.
+      rewrite <- Heq. rewrite update_pinfo_eq; auto.
+      rewrite <- Heq. rewrite update_pinfo_eq; auto.
+Qed.
+
+Lemma elim_stld_cmds_sim_wfS: forall los nts fh dones (pinfo:PhiInfo) f0 dones0 
+  main VarArgs bs1 l0 ps0 cs0 tmn0 bs2 Ps1 Ps2
   (Hpass : (f0, true, dones0) =
            elim_stld_cmds
              (fdef_intro fh (bs1 ++ block_intro l0 ps0 cs0 tmn0 :: bs2)) cs0
@@ -170,7 +384,8 @@ Lemma elim_stld_cmds_sim: forall los nts fh dones (pinfo:PhiInfo) f0 dones0 main
       (Ps1 ++
        product_fdef
          (fdef_intro fh (bs1 ++ block_intro l0 ps0 cs0 tmn0 :: bs2)) :: Ps2)]
-    main VarArgs.
+    main VarArgs /\
+  wf_system nil [module_intro los nts (Ps1 ++ product_fdef f0 :: Ps2)].
 Proof.
   intros.
   unfold elim_stld_cmds in Hpass.
@@ -178,19 +393,76 @@ Proof.
   destruct R1 as [[[[]]|[]]|]; tinv Hpass.
     remember (find_next_stld c (PI_id pinfo)) as R2.
     destruct R2 as [[|[]]|]; inv Hpass.
-      eapply las_die_sim; eauto.
-      eapply sas_sim; eauto.
-      apply program_sim_refl.
+      eapply las_die_sim_wfS; eauto.
+      split.
+        eapply sas_sim; eauto.
+        eapply sas_wfS; eauto.
+      split; auto using program_sim_refl.
 
     remember (find_next_stld c (PI_id pinfo)) as R2.
     destruct R2 as [[|[]]|]; inv Hpass.
-      eapply laa_die_sim; eauto.
-      apply program_sim_refl.
-      apply program_sim_refl.
+      eapply laa_die_sim_wfS; eauto.
+      split; auto using program_sim_refl.
+      split; auto using program_sim_refl.
 Qed.
 
-Lemma elim_stld_blocks_sim_aux: forall los nts fh dones (pinfo:PhiInfo) f0 dones0
-  main VarArgs Ps1 Ps2 flag bs2 bs1 
+Lemma elim_stld_blocks_reachablity_successors_aux: forall f0 dones0 dones id0 
+  flag fh bs2 bs1
+  (Hpass:elim_stld_blocks (fdef_intro fh (bs1++bs2)) bs2 id0 dones = 
+    (f0, flag, dones0)),
+  dtree.reachablity_analysis (fdef_intro fh (bs1++bs2)) = 
+    dtree.reachablity_analysis f0 /\
+  successors (fdef_intro fh (bs1++bs2)) = successors f0.
+Proof.
+  induction bs2; simpl; intros.
+    inv Hpass. auto.
+
+    destruct a as [l0 ps0 cs0 tmn0].
+    remember 
+      (elim_stld_cmds 
+        (fdef_intro fh (bs1 ++ block_intro l0 ps0 cs0 tmn0 :: bs2)) 
+          cs0 id0 dones) as R.
+    destruct R as [[f' []] dones']; inv Hpass; auto.
+      eapply elim_stld_cmds_reachablity_successors; eauto.
+
+      apply elim_stld_cmds_unchanged in HeqR. subst. 
+      rewrite_env ((bs1 ++ [block_intro l0 ps0 cs0 tmn0]) ++ bs2) in H0.
+      apply IHbs2 in H0; simpl_env in *; auto.
+Qed.
+
+Lemma elim_stld_blocks_wfPI_aux: forall los nts fh dones (pinfo:PhiInfo) f0 
+  dones0 Ps1 Ps2 flag bs2 bs1 
+  (Hpass:elim_stld_blocks (fdef_intro fh (bs1++bs2)) bs2 (PI_id pinfo) dones = 
+    (f0, flag, dones0))
+  (Heq: PI_f pinfo = fdef_intro fh (bs1 ++ bs2))
+  (Hwfpi: WF_PhiInfo pinfo) 
+  (HwfS : 
+     wf_system nil
+       [module_intro los nts 
+         (Ps1 ++ 
+          product_fdef 
+            (fdef_intro fh (bs1 ++ bs2)) :: Ps2)]),
+  WF_PhiInfo (update_pinfo pinfo f0).
+Proof.
+  induction bs2; simpl; intros.
+    inv Hpass.
+    rewrite <- Heq. rewrite update_pinfo_eq; auto.
+
+    destruct a as [l0 ps0 cs0 tmn0].
+    remember 
+      (elim_stld_cmds 
+        (fdef_intro fh (bs1 ++ block_intro l0 ps0 cs0 tmn0 :: bs2)) 
+          cs0 (PI_id pinfo) dones) as R.
+    destruct R as [[f' []] dones']; inv Hpass; auto.
+      eapply elim_stld_cmds_wfPI; eauto.
+
+      apply elim_stld_cmds_unchanged in HeqR. subst. 
+      rewrite_env ((bs1 ++ [block_intro l0 ps0 cs0 tmn0]) ++ bs2) in H0.
+      apply IHbs2 in H0; simpl_env in *; auto.
+Qed.
+
+Lemma elim_stld_blocks_sim_wfS_aux: forall los nts fh dones (pinfo:PhiInfo) f0 
+  dones0 main VarArgs Ps1 Ps2 flag bs2 bs1 
   (Hpass:elim_stld_blocks (fdef_intro fh (bs1++bs2)) bs2 (PI_id pinfo) dones = 
     (f0, flag, dones0))
   (Heq: PI_f pinfo = fdef_intro fh (bs1 ++ bs2))
@@ -207,10 +479,11 @@ Lemma elim_stld_blocks_sim_aux: forall los nts fh dones (pinfo:PhiInfo) f0 dones
        product_fdef f0 :: Ps2)]
     [module_intro los nts 
       (Ps1 ++ product_fdef (fdef_intro fh (bs1++bs2)) :: Ps2)]
-    main VarArgs.
+    main VarArgs /\
+   wf_system nil [module_intro los nts (Ps1 ++ product_fdef f0 :: Ps2)].
 Proof.
   induction bs2; simpl; intros.
-    inv Hpass; auto using program_sim_refl.
+    inv Hpass; split; auto using program_sim_refl.
 
     destruct a as [l0 ps0 cs0 tmn0].
     remember 
@@ -218,14 +491,44 @@ Proof.
         (fdef_intro fh (bs1 ++ block_intro l0 ps0 cs0 tmn0 :: bs2)) 
           cs0 (PI_id pinfo) dones) as R.
     destruct R as [[f' []] dones']; inv Hpass; auto.
-      eapply elim_stld_cmds_sim; eauto.
+      eapply elim_stld_cmds_sim_wfS; eauto.
 
       apply elim_stld_cmds_unchanged in HeqR. subst. 
       rewrite_env ((bs1 ++ [block_intro l0 ps0 cs0 tmn0]) ++ bs2) in H0.
       apply IHbs2 in H0; simpl_env in *; auto.
 Qed.
 
-Lemma elim_stld_blocks_sim: forall los nts fh dones (pinfo:PhiInfo) f0 dones0 
+Lemma elim_stld_blocks_reachablity_successors: forall f0 dones0 dones id0 
+  flag fh bs
+  (Hpass:elim_stld_blocks (fdef_intro fh bs) bs id0 dones = 
+    (f0, flag, dones0)),
+  dtree.reachablity_analysis (fdef_intro fh bs) = 
+    dtree.reachablity_analysis f0 /\
+  successors (fdef_intro fh bs) = successors f0.
+Proof.
+  intros.
+  rewrite_env (nil ++ bs).
+  eapply elim_stld_blocks_reachablity_successors_aux; eauto.
+Qed.
+
+Lemma elim_stld_blocks_wfPI: forall los nts fh dones (pinfo:PhiInfo) f0 dones0
+  Ps1 Ps2 flag bs 
+  (Hpass:elim_stld_blocks (fdef_intro fh bs) bs (PI_id pinfo) dones 
+           = (f0, flag, dones0))
+  (Heq: PI_f pinfo = fdef_intro fh bs)
+  (Hwfpi: WF_PhiInfo pinfo) 
+  (HwfS : 
+     wf_system nil
+       [module_intro los nts 
+         (Ps1 ++ product_fdef (fdef_intro fh bs) :: Ps2)]),
+  WF_PhiInfo (update_pinfo pinfo f0).
+Proof.
+  intros.
+  rewrite_env (nil ++ bs) in HwfS.
+  eapply elim_stld_blocks_wfPI_aux; eauto; simpl; eauto.
+Qed.
+
+Lemma elim_stld_blocks_sim_wfS: forall los nts fh dones (pinfo:PhiInfo) f0 dones0
   main VarArgs Ps1 Ps2 flag bs 
   (Hpass:elim_stld_blocks (fdef_intro fh bs) bs (PI_id pinfo) dones 
            = (f0, flag, dones0))
@@ -240,33 +543,74 @@ Lemma elim_stld_blocks_sim: forall los nts fh dones (pinfo:PhiInfo) f0 dones0
       (Ps1 ++ 
        product_fdef f0 :: Ps2)]
     [module_intro los nts (Ps1 ++ product_fdef (fdef_intro fh bs) :: Ps2)]
-    main VarArgs.
+    main VarArgs /\
+  wf_system nil [module_intro los nts (Ps1 ++ product_fdef f0 :: Ps2)].
 Proof.
   intros.
   rewrite_env (nil ++ bs).
-  eapply elim_stld_blocks_sim_aux; eauto.
+  eapply elim_stld_blocks_sim_wfS_aux; eauto.
 Qed.
 
-Lemma elim_stld_sim: forall f1 dones1 f2 dones2 Ps1 Ps2 los nts main VarArgs
-  pid (pinfo:PhiInfo) 
+Lemma elim_stld_sim_reachablity_successors: forall f1 dones1 f2 dones2 pid 
+  (Hpass: SafePrimIter.iterate _ (elim_stld_step pid) (f1, dones1) = 
+    (f2, dones2)),
+  dtree.reachablity_analysis f2 = dtree.reachablity_analysis f1 /\
+  successors f2 = successors f1.
+Proof.
+  intros. subst.
+  set (P:=fun (re:(fdef * list id)) =>
+          let '(f, _) := re in
+          dtree.reachablity_analysis f = dtree.reachablity_analysis f1 /\
+          successors f = successors f1).
+  assert (P (f1, dones1)) as HPf1.
+    unfold P. split; auto.
+  apply SafePrimIter.iterate_prop with (P:=P) in Hpass; auto.
+    unfold elim_stld_step.
+    intros a HPa.
+    destruct a as [f dones].
+    unfold elim_stld_fdef.
+    destruct f as [fh bs].
+    remember (elim_stld_blocks (fdef_intro fh bs) bs pid dones) as R.
+    destruct R as [[f0 flag0] dones0]; auto.
+    assert (P (f0, dones0)) as HPf0.
+      unfold P.
+      symmetry in HeqR.
+      apply elim_stld_blocks_reachablity_successors in HeqR.
+      destruct HeqR. destruct HPa.
+      split.
+        transitivity (dtree.reachablity_analysis (fdef_intro fh bs)); auto.
+        transitivity (successors (fdef_intro fh bs)); auto.
+
+    destruct flag0; auto.
+Qed.
+
+Lemma elim_stld_sim_wfS_wfPI: forall f1 dones1 f2 dones2 Ps1 Ps2 los nts main 
+  VarArgs pid (pinfo:PhiInfo) 
   (Hpass: SafePrimIter.iterate _ (elim_stld_step pid) 
     (f1, dones1) = (f2, dones2))
   (Heq1: PI_f pinfo = f1) (Heq2: PI_id pinfo = pid)
   (Hwfpi: WF_PhiInfo pinfo) 
   (HwfS : wf_system nil [module_intro los nts (Ps1 ++ product_fdef f1 :: Ps2)]),
-  program_sim
+  (program_sim
     [module_intro los nts (Ps1 ++ product_fdef f2 :: Ps2)]
     [module_intro los nts (Ps1 ++ product_fdef f1 :: Ps2)]
-    main VarArgs.
+    main VarArgs /\
+   wf_system nil [module_intro los nts (Ps1 ++ product_fdef f2 :: Ps2)]) /\
+  WF_PhiInfo (update_pinfo pinfo f2).
 Proof.
   intros. subst.
   set (P:=fun (re:(fdef * list id)) =>
           let '(f, _) := re in
-          program_sim [module_intro los nts (Ps1 ++ product_fdef f :: Ps2)]
-           [module_intro los nts (Ps1 ++ product_fdef (PI_f pinfo) :: Ps2)] 
-           main VarArgs).
+          (program_sim [module_intro los nts (Ps1 ++ product_fdef f :: Ps2)]
+            [module_intro los nts (Ps1 ++ product_fdef (PI_f pinfo) :: Ps2)] 
+            main VarArgs /\
+           wf_system nil
+            [module_intro los nts (Ps1 ++ product_fdef f :: Ps2)]) /\
+          WF_PhiInfo (update_pinfo pinfo f)
+       ).
   assert (P (PI_f pinfo, dones1)) as HPf1.
-    unfold P. apply program_sim_refl.
+    unfold P. 
+    split; auto using program_sim_refl.
   apply SafePrimIter.iterate_prop with (P:=P) in Hpass; auto.
     unfold elim_stld_step.
     intros a HPa.
@@ -277,35 +621,49 @@ Proof.
     destruct R as [[f0 flag0] dones0]; auto.
     assert (P (f0, dones0)) as HPf0.
       unfold P.
-      apply program_sim_trans with (P2:=
-           [module_intro los nts 
-             (Ps1 ++ product_fdef (fdef_intro fh bs) :: Ps2)]); auto.
-      eapply elim_stld_blocks_sim; eauto.
-        admit. (* PhiInfo is preserved *)
-        admit. (* wfS is preserved *)
+      symmetry in HeqR.
+      destruct HPa as [[Hsima HwfSa] HwfPIa].
+      change (PI_id pinfo) with (PI_id (update_pinfo pinfo (fdef_intro fh bs)))
+        in HeqR.
+      split.
+        apply program_sim_wfS_trans with (P2:=
+                [module_intro los nts 
+                 (Ps1 ++ product_fdef (fdef_intro fh bs) :: Ps2)]); auto.
+          intros. 
+          eapply elim_stld_blocks_sim_wfS in HeqR; eauto.
+        eapply elim_stld_blocks_wfPI in HeqR; eauto.
+
     destruct flag0; auto.
 Qed.
 
-Lemma macro_mem2reg_fdef_sim: forall rd f1 dones1 f2 dones2 Ps1 Ps2 los nts main
-  VarArgs (Hreach: ret rd = dtree.reachablity_analysis f1)
+Lemma macro_mem2reg_fdef_sim_wfS: forall rd f1 dones1 f2 dones2 Ps1 Ps2 los 
+  nts main VarArgs (Hreach: ret rd = dtree.reachablity_analysis f1)
   (HwfS : wf_system nil [module_intro los nts (Ps1 ++ product_fdef f1 :: Ps2)])
   (Hiter: SafePrimIter.iterate (fdef * list id)
             (macro_mem2reg_fdef_step rd (successors f1)
               (make_predecessors (successors f1))) 
             (f1, dones1) = (f2, dones2)),
-  program_sim
+  (program_sim
     [module_intro los nts (Ps1 ++ product_fdef f2 :: Ps2)]
     [module_intro los nts (Ps1 ++ product_fdef f1 :: Ps2)]
-    main VarArgs.
+    main VarArgs /\
+   wf_system nil [module_intro los nts (Ps1 ++ product_fdef f2 :: Ps2)]) /\
+  dtree.reachablity_analysis f1 = dtree.reachablity_analysis f2 /\
+  successors f1 = successors f2.
 Proof.
   intros.
   set (P:=fun (re:(fdef * list id)) =>
           let '(f, _) := re in
-          program_sim [module_intro los nts (Ps1 ++ product_fdef f :: Ps2)]
+          (program_sim [module_intro los nts (Ps1 ++ product_fdef f :: Ps2)]
             [module_intro los nts (Ps1 ++ product_fdef f1 :: Ps2)] main VarArgs
+          /\
+          wf_system nil
+            [module_intro los nts (Ps1 ++ product_fdef f :: Ps2)]) /\
+          dtree.reachablity_analysis f1 = dtree.reachablity_analysis f /\
+          successors f1 = successors f
       ).
   assert (P (f1, dones1)) as HPf1.
-    unfold P. apply program_sim_refl.
+    unfold P. split; auto using program_sim_refl.
   apply SafePrimIter.iterate_prop with (P:=P) in Hiter; auto.
     unfold macro_mem2reg_fdef_step.
     intros a HPa.
@@ -317,85 +675,177 @@ Proof.
     destruct R as [[[[pid ty] num] al]|]; auto.
     set (pinfo:=mkPhiInfo f rd pid ty num al).
 
-    rewrite does_stld_elim_is_true.
-      remember (SafePrimIter.iterate (fdef * list id) 
-                 (elim_stld_step pid)
-                 (phinodes_placement f rd pid ty al (successors f1)
-                 (make_predecessors (successors f1)), nil)) as R.
-      destruct R as [f0 dones0].
-      assert (P (f0, dones0)) as Pf0.
-        symmetry in HeqR1.
-        unfold P.
-        apply program_sim_trans with (P2:=
-          [module_intro los nts (Ps1 ++ 
-            product_fdef 
-               (phinodes_placement f rd pid ty al (successors f1)
-                 (make_predecessors (successors f1))) :: Ps2)]).
-          eapply elim_stld_sim with 
-            (pinfo:=mkPhiInfo (phinodes_placement f rd pid ty al (successors f1)
-                      (make_predecessors (successors f1))) rd pid ty num al); 
-            eauto.
-            admit. (* PhiInfo pres*)
-            admit. (* wfS pres*)
+    destruct HPa as [HPa [EQ2 EQ1]].
+    rewrite EQ2 in Hreach.
 
-          apply program_sim_trans with (P2:=
-            [module_intro los nts (Ps1 ++ product_fdef f :: Ps2)]); auto.
-            assert (successors f1 = successors f) as EQ1. admit. rewrite EQ1.
-            assert (dtree.reachablity_analysis f1 = 
-                      dtree.reachablity_analysis f) as EQ2.
-              admit. 
-            rewrite EQ2 in Hreach.
+    assert (WF_PhiInfo pinfo) as HwfPI.
+      eapply find_promotable_alloca__WF_PhiInfo; eauto.
+
+    rewrite does_stld_elim_is_true.
+    remember (SafePrimIter.iterate (fdef * list id) 
+               (elim_stld_step pid)
+               (phinodes_placement f rd pid ty al (successors f1)
+               (make_predecessors (successors f1)), nil)) as R.
+    destruct R as [f0 dones0].
+
+    assert (P (f0, dones0)) as HPf0.
+      symmetry in HeqR1.
+      unfold P.
+      split.
+      Case "1".
+        apply program_sim_wfS_trans with (P2:=
+            [module_intro los nts (Ps1 ++ 
+              product_fdef 
+                 (phinodes_placement f rd pid ty al (successors f1)
+                   (make_predecessors (successors f1))) :: Ps2)]); auto; intros.
+          eapply elim_stld_sim_wfS_wfPI with 
+            (pinfo:=mkPhiInfo (phinodes_placement f rd pid ty al 
+              (successors f1) (make_predecessors (successors f1))) 
+                rd pid ty num al); eauto.
+            rewrite EQ1. destruct HPa.
+            eapply phinodes_placement_wfPI; eauto.
+        
+        apply program_sim_wfS_trans with (P2:=
+          [module_intro los nts (Ps1 ++ product_fdef f :: Ps2)]); auto.
+          intros. rewrite EQ1.
+          split.
             eapply phinodes_placement_sim; eauto.
-              admit. (* wfS pres *) 
-       assert (P 
-                (if load_in_fdef pid f0 then f0 else elim_dead_st_fdef pid f0,
-                 nil)) as Pf.
-         remember (load_in_fdef pid f0) as R.
-         destruct R; auto.
-         unfold P.
-         apply program_sim_trans with (P2:=
-           [module_intro los nts (Ps1 ++ product_fdef f0 :: Ps2)]); auto.
-         apply dse_sim with (pinfo:=mkPhiInfo f0 rd pid ty num al); auto.
-           admit. (* WFPI pres *)
-           admit. (* wfS pres *)
-       remember (used_in_fdef pid
-           (if load_in_fdef pid f0 then f0 else elim_dead_st_fdef pid f0)) as R.
-       destruct R; auto.
-       apply program_sim_trans with (P2:=
-         [module_intro los nts 
-           (Ps1 ++ product_fdef 
-                     (if load_in_fdef pid f0 then f0 
-                      else elim_dead_st_fdef pid f0) :: Ps2)]); auto.
-       eapply dae_sim with 
-         (pinfo:=mkPhiInfo 
-           (if load_in_fdef pid f0 then f0 else elim_dead_st_fdef pid f0)
-           rd pid ty num al); eauto.
-         admit. (* WFPI pres *)
-         admit. (* wfS pres *)
+            eapply phinodes_placement_wfS; eauto.
+    
+      Case "2".
+        apply elim_stld_sim_reachablity_successors in HeqR1.
+        destruct HeqR1.
+        split.
+          transitivity (dtree.reachablity_analysis
+            (phinodes_placement f rd pid ty al (successors f1)
+              (make_predecessors (successors f1)))); auto.
+            rewrite EQ1. rewrite EQ2.
+            apply phinodes_placement_reachablity_analysis.
+
+          transitivity (successors
+            (phinodes_placement f rd pid ty al (successors f1)
+              (make_predecessors (successors f1)))); auto.
+            rewrite EQ1.
+
+            apply phinodes_placement_reachablity_successors.
+
+    assert (WF_PhiInfo (update_pinfo pinfo f0)) as HwfPIf0.
+      change (update_pinfo pinfo f0) with 
+             (update_pinfo 
+               (update_pinfo pinfo 
+                 (phinodes_placement f rd pid ty al (successors f)
+                   (make_predecessors (successors f)))) f0).
+     destruct HPa.
+     eapply elim_stld_sim_wfS_wfPI; eauto.
+       rewrite EQ1. simpl. auto.
+       eapply phinodes_placement_wfPI; eauto.
+         rewrite EQ1. 
+         eapply phinodes_placement_wfS; eauto.       
+
+    assert (P (if load_in_fdef pid f0 then f0 else elim_dead_st_fdef pid f0,
+              nil) /\
+            WF_PhiInfo (update_pinfo pinfo 
+              (if load_in_fdef pid f0 then f0 else elim_dead_st_fdef pid f0))) 
+      as HPf.
+      remember (load_in_fdef pid f0) as R.
+      destruct R; auto.
+      destruct HPf0 as [HPf0 HPf0'].
+      split.
+      Case "1".
+        split.
+        SCase "1.1".
+          apply program_sim_wfS_trans with (P2:=
+                  [module_intro los nts (Ps1 ++ product_fdef f0 :: Ps2)]); auto.
+            intros.
+            split; auto.
+              eapply dse_sim with (pinfo:=mkPhiInfo f0 rd pid ty num al); eauto.
+              eapply dse_wfS with (pinfo:=mkPhiInfo f0 rd pid ty num al); eauto.
+        SCase "1.2".
+          destruct HPf0' as [J1 J2].
+          split.
+            transitivity (dtree.reachablity_analysis f0); auto.
+              apply elim_dead_st_fdef_reachablity_analysis.
+            transitivity (successors f0); auto.
+              apply elim_dead_st_fdef_successors.
+
+      Case "2".  
+        destruct HPf0.
+        change (update_pinfo pinfo (elim_dead_st_fdef pid f0)) with 
+                 (update_pinfo 
+                   (update_pinfo 
+                     (update_pinfo pinfo
+                       (phinodes_placement f rd pid ty al (successors f)
+                         (make_predecessors (successors f)))) 
+                   f0)
+                   (elim_dead_st_fdef pid f0)
+                 ).
+        eapply dse_wfPI; eauto.
+
+    destruct HPf as [HPf HwfPI0].
+    remember (used_in_fdef pid
+        (if load_in_fdef pid f0 then f0 else elim_dead_st_fdef pid f0)) as R.
+    destruct R; auto.
+    destruct HPf as [HPf HPf'].
+    split.
+      apply program_sim_wfS_trans with (P2:=
+                 [module_intro los nts 
+                   (Ps1 ++ product_fdef 
+                   (if load_in_fdef pid f0 then f0 
+                    else elim_dead_st_fdef pid f0) :: Ps2)]); auto.
+        intros. 
+        split.
+          eapply dae_sim with 
+            (pinfo:=mkPhiInfo 
+              (if load_in_fdef pid f0 then f0 else elim_dead_st_fdef pid f0)
+              rd pid ty num al); eauto.
+          eapply dae_wfS with 
+            (pinfo:=mkPhiInfo 
+              (if load_in_fdef pid f0 then f0 else elim_dead_st_fdef pid f0)
+              rd pid ty num al); eauto.
+
+      destruct HPf' as [Hreach' Hsucc'].
+      split.
+        transitivity 
+          (dtree.reachablity_analysis
+            (if load_in_fdef pid f0 then f0 else elim_dead_st_fdef pid f0));auto.
+        apply remove_reachablity_analysis; auto.
+
+        transitivity 
+          (successors
+            (if load_in_fdef pid f0 then f0 else elim_dead_st_fdef pid f0));auto.
+        apply remove_successors; auto.
 Qed.
 
-Lemma eliminate_phis_sim: forall f Ps1 Ps2 los nts main VarArgs,
+Lemma eliminate_phis_sim_wfS: forall f Ps1 Ps2 los nts main VarArgs
+  (HwfS : wf_system nil [module_intro los nts (Ps1 ++ product_fdef f :: Ps2)]),
   program_sim
     [module_intro los nts 
       (Ps1 ++ product_fdef (SafePrimIter.iterate fdef eliminate_step f) :: Ps2)]
     [module_intro los nts (Ps1 ++ product_fdef f :: Ps2)]
-    main VarArgs.
-Admitted.
+    main VarArgs /\
+  wf_system nil 
+    [module_intro los nts 
+      (Ps1 ++ product_fdef (SafePrimIter.iterate fdef eliminate_step f) :: Ps2)].
+Admitted. (* From previous work *)
 
-Axiom fix_temporary_fdef_sim: forall f1 f2 Ps1 Ps2 los nts main VarArgs
-  (Hpass: ret f2 = fix_temporary_fdef f1),
+Axiom fix_temporary_fdef_sim_wfS: forall f1 f2 Ps1 Ps2 los nts main VarArgs
+  (Hpass: ret f2 = fix_temporary_fdef f1)
+  (HwfS : wf_system nil [module_intro los nts (Ps1 ++ product_fdef f1 :: Ps2)]),
   program_sim
     [module_intro los nts (Ps1 ++ product_fdef f2 :: Ps2)]
     [module_intro los nts (Ps1 ++ product_fdef f1 :: Ps2)]
-    main VarArgs.
+    main VarArgs /\
+  wf_system nil [module_intro los nts (Ps1 ++ product_fdef f2 :: Ps2)].
 
-Lemma mem2reg_fdef_sim: forall (main : id) (VarArgs : list (GVsT DGVs))
+Lemma mem2reg_fdef_sim_wfS: forall (main : id) (VarArgs : list (GVsT DGVs))
   (los : layouts) (nts : namedts) (f : fdef) (Ps2 Ps1 : products)
- (HwfS : wf_system nil [module_intro los nts (Ps1 ++ product_fdef f :: Ps2)]),
+  (HwfS : wf_system nil [module_intro los nts (Ps1 ++ product_fdef f :: Ps2)]),
   program_sim
     [module_intro los nts (Ps1 ++ product_fdef (mem2reg_fdef f) :: Ps2)]
     [module_intro los nts (Ps1 ++ product_fdef f :: Ps2)]
-    main VarArgs.
+    main VarArgs /\
+  wf_system nil 
+    [module_intro los nts (Ps1 ++ product_fdef (mem2reg_fdef f) :: Ps2)].
 Proof.
   intros.
   unfold mem2reg_fdef.
@@ -414,19 +864,19 @@ Proof.
   remember (fix_temporary_fdef (SafePrimIter.iterate fdef eliminate_step f1))
     as R.
   destruct R as [f2|]; auto using program_sim_refl.
-  apply program_sim_trans with (P2:=
-    [module_intro los nts (Ps1 ++ product_fdef f1 :: Ps2)]).
-    apply program_sim_trans with (P2:=
+  apply program_sim_wfS_trans with (P2:=
+    [module_intro los nts (Ps1 ++ product_fdef f1 :: Ps2)]); auto; intros.
+    apply program_sim_wfS_trans with (P2:=
       [module_intro los nts 
         (Ps1 ++ product_fdef (SafePrimIter.iterate fdef eliminate_step f1) 
-          :: Ps2)]).
-      eapply fix_temporary_fdef_sim; eauto.
-      apply eliminate_phis_sim; auto.
+          :: Ps2)]); auto; intros.
+      eapply fix_temporary_fdef_sim_wfS; eauto.
+      apply eliminate_phis_sim_wfS; auto.
 
-    eapply macro_mem2reg_fdef_sim; eauto.
+    eapply macro_mem2reg_fdef_sim_wfS; eauto.
 Qed.
 
-Lemma mem2reg_run_sim_aux: forall (main : id) (VarArgs : list (GVsT DGVs))        
+Lemma mem2reg_run_sim_wfS_aux: forall (main : id) (VarArgs : list (GVsT DGVs))   
   (los : layouts) (nts : namedts) (Ps2 Ps1: products)
   (HwfS : wf_system nil [module_intro los nts (Ps1 ++ Ps2)]),
   program_sim
@@ -436,34 +886,41 @@ Lemma mem2reg_run_sim_aux: forall (main : id) (VarArgs : list (GVsT DGVs))
           match p with
           | product_fdef f => product_fdef (mem2reg_fdef f)
           | _ => p
-          end) Ps2)] [module_intro los nts (Ps1++Ps2)] main VarArgs.
+          end) Ps2)] [module_intro los nts (Ps1++Ps2)] main VarArgs /\
+  wf_system nil
+    [module_intro los nts
+      (Ps1 ++ List.map
+        (fun p : product =>
+          match p with
+          | product_fdef f => product_fdef (mem2reg_fdef f)
+          | _ => p
+          end) Ps2)].
 Proof.
   induction Ps2; simpl; intros.
-    apply program_sim_refl.
+    split; auto using program_sim_refl.
 
     assert (J:=@IHPs2 (Ps1 ++ [a])). clear IHPs2.
     simpl_env in J. simpl in J. 
     destruct a; auto.
-    apply program_sim_trans with (P2:=
+    apply program_sim_wfS_trans with (P2:=
       [module_intro los nts
         (Ps1 ++ product_fdef f :: 
            List.map (fun p : product =>
                      match p with
                      | product_fdef f => product_fdef (mem2reg_fdef f)
                      | _ => p
-                     end) Ps2)]); auto.
-    apply mem2reg_fdef_sim.
-      admit. (* wfS pres *)
+                     end) Ps2)]); auto; intros.
+    apply mem2reg_fdef_sim_wfS; auto.
 Qed.
 
-Lemma mem2reg_run_sim: forall (m:module) (main:id) (VarArgs:list (GVsT DGVs))
+Lemma mem2reg_run_sim_wfS: forall (m:module) (main:id) (VarArgs:list (GVsT DGVs))
   (HwfS : wf_system nil [m]),
-  program_sim [mem2reg.run m] [m] main VarArgs.
+  program_sim [mem2reg.run m] [m] main VarArgs /\ wf_system nil [mem2reg.run m].
 Proof.
   destruct m as [los nts Ps].
   unfold mem2reg.run.
   intros.
-  assert (J:=@mem2reg_run_sim_aux main VarArgs los nts Ps nil).
+  assert (J:=@mem2reg_run_sim_wfS_aux main VarArgs los nts Ps nil).
   auto.
 Qed.
 
